theories/rules/rules_base.v
@@ -110,8 +110,9 @@ Section cap_lang_rules.
 
   (* Conditionally unify on the read register value *)
   Definition read_reg_inr  (regs : Reg) (r : RegName) p b e a :=
-    regs !! r = Some (inr (p, b, e, a)) ∨ ∃ z, regs !! r = Some(inl z).
-
+    match regs !! r with
+      | Some w => get_cap w = Some (p,b,e,a) ∨ get_cap w = None
+      | None => False end.
 
   (* ------------------------- registers points-to --------------------------------- *)
 
@@ -525,7 +526,7 @@ Section cap_lang_rules.
 
   Lemma wp_notCorrectPC_perm E pc_p pc_b pc_e pc_a :
       pc_p ≠ RX ∧ pc_p ≠ RWX →
-      {{{ PC ↦ᵣ inr (pc_p,pc_b,pc_e,pc_a)}}}
+      {{{ PC ↦ᵣ put_cap (pc_p,pc_b,pc_e,pc_a)}}}
       Instr Executable @ E
       {{{ RET FailedV; True }}}.
   Proof.
@@ -538,7 +539,7 @@ Section cap_lang_rules.
 
   Lemma wp_notCorrectPC_range E pc_p pc_b pc_e pc_a :
        ¬ (pc_b <= pc_a < pc_e)%a →
-      {{{ PC ↦ᵣ inr (pc_p,pc_b,pc_e,pc_a)}}}
+      {{{ PC ↦ᵣ put_cap (pc_p,pc_b,pc_e,pc_a)}}}
       Instr Executable @ E
       {{{ RET FailedV; True }}}.
   Proof.
@@ -553,11 +554,11 @@ Section cap_lang_rules.
 
   Lemma wp_halt E pc_p pc_b pc_e pc_a w :
     decodeInstrW w = Halt →
-    isCorrectPC (inr (pc_p,pc_b,pc_e,pc_a)) →
+    isCorrectPC (put_cap (pc_p,pc_b,pc_e,pc_a)) →
 
-    {{{ PC ↦ᵣ inr (pc_p,pc_b,pc_e,pc_a) ∗ pc_a ↦ₐ w }}}
+    {{{ PC ↦ᵣ put_cap (pc_p,pc_b,pc_e,pc_a) ∗ pc_a ↦ₐ w }}}
       Instr Executable @ E
-    {{{ RET HaltedV; PC ↦ᵣ inr (pc_p,pc_b,pc_e,pc_a) ∗ pc_a ↦ₐ w }}}.
+    {{{ RET HaltedV; PC ↦ᵣ put_cap (pc_p,pc_b,pc_e,pc_a) ∗ pc_a ↦ₐ w }}}.
   Proof.
     intros Hinstr Hvpc.
     iIntros (φ) "[Hpc Hpca] Hφ".
@@ -576,11 +577,11 @@ Section cap_lang_rules.
 
   Lemma wp_fail E pc_p pc_b pc_e pc_a w :
     decodeInstrW w = Fail →
-    isCorrectPC (inr (pc_p,pc_b,pc_e,pc_a)) →
+    isCorrectPC (put_cap (pc_p,pc_b,pc_e,pc_a)) →
 
-    {{{ PC ↦ᵣ inr (pc_p,pc_b,pc_e,pc_a) ∗ pc_a ↦ₐ w }}}
+    {{{ PC ↦ᵣ put_cap (pc_p,pc_b,pc_e,pc_a) ∗ pc_a ↦ₐ w }}}
       Instr Executable @ E
-    {{{ RET FailedV; PC ↦ᵣ inr (pc_p,pc_b,pc_e,pc_a) ∗ pc_a ↦ₐ w }}}.
+    {{{ RET FailedV; PC ↦ᵣ put_cap (pc_p,pc_b,pc_e,pc_a) ∗ pc_a ↦ₐ w }}}.
   Proof.
     intros Hinstr Hvpc.
     iIntros (φ) "[Hpc Hpca] Hφ".
@@ -638,8 +639,8 @@ Ltac iFailWP Hcont fail_case_name :=
 (*--- register equality ---*)
   Lemma addr_ne_reg_ne {regs : leibnizO Reg} {r1 r2 : RegName}
         {p0 b0 e0 a0 p b e a}:
-    regs !! r1 = Some (inr (p0,  b0, e0, a0))
-    → regs !! r2 = Some (inr (p, b, e, a))
+    regs !! r1 = Some (put_cap (p0,  b0, e0, a0))
+    → regs !! r2 = Some (put_cap (p, b, e, a))
     → a0 ≠ a → r1 ≠ r2.
   Proof.
     intros Hr1 Hr2 Hne.
@@ -650,13 +651,13 @@ Ltac iFailWP Hcont fail_case_name :=
 
 Definition word_of_argument (regs: Reg) (a: Z + RegName): option Word :=
   match a with
-  | inl n => Some (inl n)
+  | inl n => Some (put_z n)
   | inr r => regs !! r
   end.
 
 Lemma word_of_argument_Some_inv (regs: Reg) (arg: Z + RegName) (w:Word) :
   word_of_argument regs arg = Some w →
-  ((∃ z, arg = inl z ∧ w = inl z) ∨
+  ((∃ z, arg = inl z ∧ w = put_z z) ∨
    (∃ r, arg = inr r ∧ regs !! r = Some w)).
 Proof.
   unfold word_of_argument. intro. repeat case_match; simplify_eq/=; eauto.
@@ -665,12 +666,24 @@ Qed.
 Lemma word_of_argument_Some_inv' (regs regs': Reg) (arg: Z + RegName) (w:Word) :
   word_of_argument regs arg = Some w →
   regs ⊆ regs' →
-  ((∃ z, arg = inl z ∧ w = inl z) ∨
+  ((∃ z, arg = inl z ∧ w = put_z z) ∨
    (∃ r, arg = inr r ∧ regs !! r = Some w ∧ regs' !! r = Some w)).
 Proof.
   unfold word_of_argument. intro. repeat case_match; simplify_eq/=; eauto.
   intros HH. unshelve epose proof (lookup_weaken _ _ _ _ _ HH); eauto.
 Qed.
+
+  Lemma word_of_argument_inr (regs: Reg) (arg: Z + RegName) (c0 : Cap):
+    word_of_argument regs arg = Some(put_cap c0) →
+    (∃ r : RegName, arg = inr r ∧ regs !! r = Some(put_cap c0)).
+  Proof.
+    intros HStoreV.
+    unfold word_of_argument in HStoreV.
+    destruct arg.
+       - by inversion HStoreV.
+       - exists r. destruct (regs !! r) eqn:Hvr0; last by inversion HStoreV.
+         split; auto.
+  Qed.
 
 (*--- addr_of_argument ---*)
 
@@ -683,7 +696,7 @@ Definition addr_of_argument regs src :=
 Lemma addr_of_argument_Some_inv (regs: Reg) (arg: Z + RegName) (a:Addr) :
   addr_of_argument regs arg = Some a →
   ∃ z, z_to_addr z = Some a ∧
-       (arg = inl z ∨ ∃ r, arg = inr r ∧ regs !! r = Some (inl z)).
+       (arg = inl z ∨ ∃ r, arg = inr r ∧ regs !! r = Some (put_z z)).
 Proof.
   unfold addr_of_argument, z_of_argument.
   intro. repeat case_match; simplify_eq/=; eauto. eexists. eauto.
@@ -693,7 +706,7 @@ Lemma addr_of_argument_Some_inv' (regs regs': Reg) (arg: Z + RegName) (a:Addr) :
   addr_of_argument regs arg = Some a →
   regs ⊆ regs' →
   ∃ z, z_to_addr z = Some a ∧
-       (arg = inl z ∨ ∃ r, arg = inr r ∧ regs !! r = Some (inl z) ∧ regs' !! r = Some (inl z)).
+       (arg = inl z ∨ ∃ r, arg = inr r ∧ regs !! r = Some (put_z z) ∧ regs' !! r = Some (put_z z)).
 Proof.
   unfold addr_of_argument, z_of_argument.
   intros ? HH. repeat case_match; simplify_eq/=; eauto. eexists. split; eauto.
@@ -725,6 +738,8 @@ Definition regs_of (i: instr): gset RegName :=
   | Load r1 r2 => {[ r1; r2 ]}
   | Store r1 arg => {[ r1 ]} ∪ regs_of_argument arg
   | Jnz r1 r2 => {[ r1; r2 ]}
+  | Seal dst r1 r2 => {[dst; r1; r2]}
+  | UnSeal dst r1 r2 => {[dst; r1; r2]}
   | _ => ∅
   end.
 
@@ -745,9 +760,9 @@ Qed.
 
 Definition incrementPC (regs: Reg) : option Reg :=
   match regs !! PC with
-  | Some (inr (p, b, e, a)) =>
+  | Some (put_cap (p, b, e, a)) =>
     match (a + 1)%a with
-    | Some a' => Some (<[ PC := inr (p, b, e, a') ]> regs)
+    | Some a' => Some (<[ PC := put_cap (p, b, e, a') ]> regs)
     | None => None
     end
   | _ => None
@@ -756,26 +771,26 @@ Definition incrementPC (regs: Reg) : option Reg :=
 Lemma incrementPC_Some_inv regs regs' :
   incrementPC regs = Some regs' ->
   exists p b e a a',
-    regs !! PC = Some (inr (p, b, e, a)) ∧
+    regs !! PC = Some (put_cap (p, b, e, a)) ∧
     (a + 1)%a = Some a' ∧
-    regs' = <[ PC := inr (p, b, e, a') ]> regs.
+    regs' = <[ PC := put_cap (p, b, e, a') ]> regs.
 Proof.
   unfold incrementPC.
-  destruct (regs !! PC) as [ [| [ [ [ ? ?] ?] u] ] |];
-    try congruence.
-  case_eq (u+1)%a; try congruence. intros ? ?. inversion 1.
-  do 5 eexists. split; eauto.
+  destruct (regs !! PC) as [w|]; last congruence.
+  destruct_word w; try congruence. destruct_cap c.
+  destruct (_ + 1)%a eqn:Heq; last congruence. inversion 1.
+  repeat eexists. done.
 Qed.
 
 Lemma incrementPC_None_inv regs pg b e a :
   incrementPC regs = None ->
-  regs !! PC = Some (inr (pg, b, e, a)) ->
+  regs !! PC = Some (put_cap (pg, b, e, a)) ->
   (a + 1)%a = None.
 Proof.
   unfold incrementPC.
-  destruct (regs !! PC) as [ [| [ [ [ ? ?] ?] u] ] |];
-    try congruence.
-  case_eq (u+1)%a; congruence.
+  destruct (regs !! PC) as [w|]; last congruence.
+  destruct_word w; try congruence. destruct_cap c.
+  destruct (_+1)%a eqn:HSome; congruence.
 Qed.
 
 Lemma incrementPC_overflow_mono regs regs' :
@@ -787,8 +802,8 @@ Proof.
   intros Hi HPC Hincl. unfold incrementPC in *. destruct HPC as [c HPC].
   pose proof (lookup_weaken _ _ _ _ HPC Hincl) as HPC'.
   rewrite HPC HPC' in Hi |- *.
-  destruct c as [| (((?&?)&?)&aa)]; first by auto.
-  destruct (aa+1)%a; last by auto. congruence.
+  destruct_word c; auto.
+  destruct_cap c0; destruct (_ + 1)%a; auto. congruence.
 Qed.
 
 (* todo: instead, define updatePC on top of incrementPC *)
@@ -798,22 +813,22 @@ Lemma incrementPC_fail_updatePC regs m :
 Proof.
    rewrite /incrementPC /updatePC /RegLocate /=.
    destruct (regs !! PC) as [X|]; auto.
-   destruct X as [| [[[? ?] ?] a']]; auto.
-   destruct (a' + 1)%a; auto. congruence.
+   destruct_word X; auto. destruct_cap c.
+   destruct (_ + 1)%a; auto. congruence.
 Qed.
 
 Lemma incrementPC_success_updatePC regs m regs' :
   incrementPC regs = Some regs' ->
   ∃ p b e a a',
-    regs !! PC = Some (inr ((p, b, e, a))) ∧
+    regs !! PC = Some (put_cap (p, b, e, a)) ∧
     (a + 1)%a = Some a' ∧
-    updatePC (regs, m) = (NextI, (<[ PC := inr (p, b, e, a') ]> regs, m)) ∧
-    regs' = <[ PC := inr (p, b, e, a') ]> regs.
+    updatePC (regs, m) = (NextI, (<[ PC := put_cap (p, b, e, a') ]> regs, m)) ∧
+    regs' = <[ PC := put_cap (p, b, e, a') ]> regs.
 Proof.
   rewrite /incrementPC /updatePC /update_reg /RegLocate /=.
   destruct (regs !! PC) as [X|] eqn:?; auto; try congruence; [].
-  destruct X as [| [[[? ?] ?] a']] eqn:?; try congruence; [].
-  destruct (a' + 1)%a eqn:?; [| congruence]. inversion 1; subst regs'.
+  destruct_word X; try congruence. destruct_cap c.
+  destruct (_ + 1)%a eqn:?; [| congruence]. inversion 1; subst regs'.
   do 5 eexists. repeat split; auto.
 Qed.
 
@@ -826,8 +841,8 @@ Proof.
   destruct (regs !! PC) as [ w1 |] eqn:Hrr.
   { pose proof (regs_lookup_eq _ _ _ Hrr) as Hrr2. rewrite Hrr2 in Hu.
     pose proof (lookup_weaken _ _ _ _ Hrr Hincl) as ->%regs_lookup_eq.
-    destruct w1 as [|(((?&?)&?)&a1)]; simplify_eq.
-    destruct (a1 + 1)%a eqn:Ha1; simplify_eq. rewrite /update_reg /=.
+    destruct_word w1; try congruence. destruct_cap c; subst.
+    destruct (_ + 1)%a eqn:Ha1; simplify_eq. rewrite /update_reg /=.
     f_equal. f_equal.
     assert (HH: forall (reg1 reg2:Reg), reg1 = reg2 -> reg1 !! PC = reg2 !! PC)
       by (intros * ->; auto).
@@ -843,8 +858,8 @@ Lemma updatePC_fail_incl m m' regs regs' :
 Proof.
   intros [w HPC] Hincl Hfail. rewrite /updatePC /RegLocate /= in Hfail |- *.
   rewrite !HPC in Hfail. have -> := lookup_weaken _ _ _ _ HPC Hincl.
-  destruct w as [|(((?&?)&?)&a1)]; simplify_eq; auto;[].
-  destruct (a1 + 1)%a; simplify_eq; auto.
+  destruct_word w; simplify_eq; auto;[].
+  destruct_cap c. destruct (_ + 1)%a; simplify_eq; auto.
 Qed.
 
 Ltac incrementPC_inv :=
